extra credit (option 2) for final (lean)

final/lean/program/Final/arith_var.lean
@@ -5,7 +5,8 @@ example : Binop := Binop.Add
 inductive Expr
 | Num : Nat → Expr
 | Binop : Binop → Expr → Expr → Expr
--- Fill in Let and Var syntax
+| Let : Expr → Expr → Expr
+| Var : Nat → Expr
 
 example : Expr := Expr.Num 1
 example : Expr := Expr.Binop Binop.Add (Expr.Num 1) (Expr.Num 2)
@@ -21,11 +22,17 @@ def apply_binop (op : Binop) (nl nr : Nat) : Nat :=
   Binop.casesOn op (nl + nr) (nl - nr) (nl * nr) (nl / nr)
 
 inductive subst : Nat → Expr → Expr → Expr → Prop
-| SNum (i n : Nat) (e' : Expr) : subst i e' (Expr.Num n) (Expr.Num n)
-| SBinop (op : Binop) (i : Nat) (el er el' er' e' : Expr) :
+| SNum {i n : Nat} {e' : Expr} : subst i e' (Expr.Num n) (Expr.Num n)
+| SBinop {op : Binop} {i : Nat} {el er el' er' e' : Expr} :
   subst i e' el el' → subst i e' er er' →
   subst i e' (Expr.Binop op el er) (Expr.Binop op el' er')
--- Fill in remaining substitution rules
+| SLet {i : Nat} {e' evar ebody evar' ebody' : Expr} :
+  subst i e' evar evar' → subst (i + 1) e' ebody ebody' →
+  subst i e' (Expr.Let evar ebody) (Expr.Let evar' ebody')
+| SVarEq {i : Nat} {e' : Expr} :
+  subst i e' (Expr.Var i) e'
+| SVarNe {i j : Nat} {e' : Expr} :
+  i > j → subst i e' (Expr.Var j) (Expr.Var j)
 
 inductive steps : Expr → Expr → Prop
 | DLeft (op : Binop) (el el' er : Expr) :
@@ -42,26 +49,91 @@ inductive steps : Expr → Expr → Prop
   steps
     (Expr.Binop op (Expr.Num nl) (Expr.Num nr))
     (Expr.Num (apply_binop op nl nr))
--- Fill in D-Let step rule
+| DLet (evar ebody ebody' : Expr) :
+  subst 0 evar ebody ebody' →
+  steps (Expr.Let evar ebody) ebody'
 
 notation:35 e " ↦ " e' => steps e e'
 
 example : (Expr.Binop Binop.Add (Expr.Num 1) (Expr.Num 2)) ↦ (Expr.Num 3) :=
-   steps.DOp Binop.Add 1 2
+  steps.DOp Binop.Add 1 2
+
+-- let 2 in ((var 0) + 3) ↦ 2 + 3
+example : (Expr.Let (Expr.Num 2) (Expr.Binop Binop.Add (Expr.Var 0) (Expr.Num 3)))
+            ↦ (Expr.Binop Binop.Add (Expr.Num 2) (Expr.Num 3)) := by
+  apply steps.DLet
+  apply subst.SBinop
+  apply subst.SVarEq
+  apply subst.SNum
 
 inductive valid : Nat → Expr → Prop
-| TNum (n i : Nat) :
-  valid i (Expr.Num n)
-| TBinop (op : Binop) (el er : Expr) (i : Nat) :
-  valid i el → valid i er → valid i (Expr.Binop op el er)
--- Fill in T-Let and T-Var rules
+| TNum {n ctx : Nat} :
+  valid ctx (Expr.Num n)
+| TBinop {op : Binop} {el er : Expr} {ctx : Nat} :
+  valid ctx el → valid ctx er → valid ctx (Expr.Binop op el er)
+| TLet {ctx : Nat} {evar ebody : Expr} :
+  valid ctx evar → valid (ctx + 1) ebody → valid ctx (Expr.Let evar ebody)
+| TVar {ctx i : Nat} :
+  i < ctx → valid ctx (Expr.Var i)
 
+theorem valid_in_bigger_context {e : Expr} {i : Nat} :
+    valid i e → valid (i + 1) e := by
+  intro hvalid
+  induction hvalid
+  case TNum => apply valid.TNum
+  case TBinop hl hr ihl ihr =>
+    apply valid.TBinop ihl ihr
+  case TLet hvar hbody ihvar ihbody =>
+    simp at ihbody
+    apply valid.TLet ihvar ihbody
+  case TVar ctx var ihle =>
+    apply valid.TVar
+    have h : ctx < ctx + 1 := by simp
+    apply Trans.trans ihle h
 
-theorem subst_preserves_valid :
-  ∀ (e e' esub : Expr), ∀ (i : Nat),
-    valid (i+1) e → valid i e' → subst i e' e esub → valid i esub :=
-  sorry -- Remove this line and add your proof
+theorem subst_preserves_valid {ebody evar esub : Expr} {ctx : Nat} :
+    valid (ctx + 1) ebody → valid ctx evar → subst ctx evar ebody esub → valid ctx esub := by
+  intro hvbody hvvar hsubst
+  induction hsubst
+  case SNum n => apply valid.TNum
+  case SBinop hl hr ihl ihr =>
+    apply valid.TBinop
+    match hvbody with | valid.TBinop hl' _ => apply ihl hl' hvvar
+    match hvbody with | valid.TBinop _ hr' => apply ihr hr' hvvar
+  case SLet i e' _ _ _ _ hvar hbody ihvar ihbody =>
+    apply valid.TLet
+    match hvbody with | valid.TLet v _ => apply ihvar v hvvar
+    match hvbody with
+    | valid.TLet _ b =>
+      apply ihbody b (valid_in_bigger_context hvvar)
+  case SVarEq => apply hvvar
+  case SVarNe =>
+    apply valid.TVar
+    assumption
+
 
 theorem preservation :
-  ∀ e e' : Expr, (e ↦ e') → valid 0 e → valid 0 e' :=
-  sorry -- Remove this line and add your proof
+    ∀ e e' : Expr, (e ↦ e') → valid 0 e → valid 0 e' := by
+  intro e e' hstep hvalid
+  cases e
+  case Num n => contradiction
+  case Binop op el er =>
+    cases hstep
+    case DLeft el' h =>
+      apply valid.TBinop
+      apply preservation el el' h
+      match hvalid with | valid.TBinop h1 _ => exact h1
+      match hvalid with | valid.TBinop _ h2 => exact h2
+    case DRight er' v h =>
+      apply valid.TBinop
+      match hvalid with | valid.TBinop h1 _ => exact h1
+      apply preservation er er' h
+      match hvalid with | valid.TBinop _ h2 => exact h2
+    case DOp nl nr => apply valid.TNum
+  case Let evar ebody =>
+    cases hstep
+    case DLet hsubst =>
+      apply subst_preserves_valid _ _ hsubst
+      match hvalid with | valid.TLet _ b => exact b
+      match hvalid with | valid.TLet v _ => exact v
+  case Var i => contradiction
